Optimizations/Canonicalizations/Common.thy
@@ -4,19 +4,7 @@ theory Common
   imports 
     OptimizationDSL.Canonicalization
     Semantics.IRTreeEvalThms
-    "HOL-Eisbach.Eisbach"
 begin
-
-fun size :: "IRExpr \<Rightarrow> nat" where
-  "size (UnaryExpr op e) = (size e) + 1" |
-  "size (BinaryExpr BinAdd x y) = (size x) + ((size y) * 2)" |
-  "size (BinaryExpr op x y) = (size x) + (size y)" |
-  "size (ConditionalExpr cond t f) = (size cond) + (size t) + (size f) + 2" |
-  "size (ConstantExpr c) = 1" |
-  "size (ParameterExpr ind s) = 2" |
-  "size (LeafExpr nid s) = 2" |
-  "size (ConstantVar c) = 2" |
-  "size (VariableExpr x s) = 2"
 
 lemma size_pos[simp]: "0 < size y"
   apply (induction y; auto?)
@@ -35,12 +23,5 @@ lemma size_non_const:
     using size_non_add size_pos apply auto
     by (simp add: Suc_lessI one_is_add)+
   done
-
-method unfold_optimization =
-  (unfold rewrite_preservation.simps, unfold rewrite_termination.simps,
-    unfold intval.simps,
-    rule conjE, simp, simp del: le_expr_def)
-  | (unfold rewrite_preservation.simps, unfold rewrite_termination.simps,
-    rule conjE, simp, simp del: le_expr_def)
 
 end
