Optimizations/DSL/Canonicalization.thy
@@ -4,6 +4,7 @@ theory Canonicalization
   imports
     Markup
     Phase
+    "HOL-Eisbach.Eisbach"
   keywords
     "phase" :: thy_decl and 
     "terminating" :: quasi_command and
@@ -91,6 +92,30 @@ fun intval :: "Value Rewrite \<Rightarrow> bool" where
   "intval (Conditional x y cond) = (cond \<longrightarrow> (x = y))" |
   "intval (Sequential x y) = (intval x \<and> intval y)" |
   "intval (Transitive x) = intval x"
+
+fun size :: "IRExpr \<Rightarrow> nat" where
+  "size (UnaryExpr op e) = (size e) + 1" |
+  "size (BinaryExpr BinAdd x y) = (size x) + ((size y) * 2)" |
+  "size (BinaryExpr op x y) = (size x) + (size y)" |
+  "size (ConditionalExpr cond t f) = (size cond) + (size t) + (size f) + 2" |
+  "size (ConstantExpr c) = 1" |
+  "size (ParameterExpr ind s) = 2" |
+  "size (LeafExpr nid s) = 2" |
+  "size (ConstantVar c) = 2" |
+  "size (VariableExpr x s) = 2"
+
+method unfold_optimization =
+  (unfold rewrite_preservation.simps, unfold rewrite_termination.simps,
+    unfold intval.simps,
+    rule conjE, simp, simp del: le_expr_def, force?)
+  | (unfold rewrite_preservation.simps, unfold rewrite_termination.simps,
+    rule conjE, simp, simp del: le_expr_def, force?)
+
+method unfold_size =
+  (unfold size.simps, simp del: le_expr_def)?
+  | (unfold size.simps)?
+
+print_methods
 
 ML \<open>
 structure System : RewriteSystem =
