Semantics/TreeToGraph.thy
@@ -169,6 +169,7 @@ inductive
     \<Longrightarrow> g \<turnstile> n \<simeq> e"
 
 code_pred (modes: i \<Rightarrow> i \<Rightarrow> o \<Rightarrow> bool as exprE) rep .
+code_pred (modes: i \<Rightarrow> o \<Rightarrow> i \<Rightarrow> bool as exprE) rep .
 
 
 inductive
@@ -326,77 +327,56 @@ value "get_fresh_id (add_node 6 (ParameterNode 2, default_stamp) eg2_sq)"
 
    This means that we can try to re-use existing nodes by finding node IDs bottom-up.
 *)
+
+(* TODO: document distinction between unrep and add_expr *)
 inductive
   unrep :: "IRGraph \<Rightarrow> IRExpr \<Rightarrow> (IRGraph \<times> ID) \<Rightarrow> bool" ("_ \<oplus> _ \<leadsto> _" 55)
-   where
+  and
+  add_expr :: "IRGraph \<Rightarrow> IRExpr \<Rightarrow> (IRGraph \<times> ID) \<Rightarrow> bool"
+  where
 
-  ConstantNodeSame:
-  "\<lbrakk>find_node_and_stamp g (ConstantNode c, constantAsStamp c) = Some n\<rbrakk>
-    \<Longrightarrow> g \<oplus> (ConstantExpr c) \<leadsto> (g, n)" |
+  Exists:
+  "\<lbrakk>g \<turnstile> n \<simeq> e\<rbrakk>
+    \<Longrightarrow> g \<oplus> e \<leadsto> (g, n)" |
+
+  NotExists:
+  "\<lbrakk>\<not>(\<exists>n. (g \<turnstile> n \<simeq> e));
+    add_expr g e (g', n')\<rbrakk>
+    \<Longrightarrow> g \<oplus> e \<leadsto> (g', n')" |
 
   ConstantNodeNew:
-  "\<lbrakk>find_node_and_stamp g (ConstantNode c, constantAsStamp c) = None;
-    n = get_fresh_id g;
+  "\<lbrakk>n = get_fresh_id g;
     g' = add_node n (ConstantNode c, constantAsStamp c) g \<rbrakk>
-    \<Longrightarrow> g \<oplus> (ConstantExpr c) \<leadsto> (g', n)" |
-
-  ParameterNodeSame:
-  "\<lbrakk>find_node_and_stamp g (ParameterNode i, s) = Some n\<rbrakk>
-    \<Longrightarrow> g \<oplus> (ParameterExpr i s) \<leadsto> (g, n)" |
+    \<Longrightarrow> add_expr g (ConstantExpr c) (g', n)" |
 
   ParameterNodeNew:
-  "\<lbrakk>find_node_and_stamp g (ParameterNode i, s) = None;
-    n = get_fresh_id g;
+  "\<lbrakk>n = get_fresh_id g;
     g' = add_node n (ParameterNode i, s) g\<rbrakk>
-    \<Longrightarrow> g \<oplus> (ParameterExpr i s) \<leadsto> (g', n)" |
-
-  ConditionalNodeSame:
-  "\<lbrakk>g \<oplus> ce \<leadsto> (g2, c);
-    g2 \<oplus> te \<leadsto> (g3, t);
-    g3 \<oplus> fe \<leadsto> (g4, f);
-    s' = meet (stamp g4 t) (stamp g4 f);
-    find_node_and_stamp g4 (ConditionalNode c t f, s') = Some n\<rbrakk>
-    \<Longrightarrow> g \<oplus> (ConditionalExpr ce te fe) \<leadsto> (g4, n)" |
+    \<Longrightarrow> add_expr g (ParameterExpr i s) (g', n)" |
 
   ConditionalNodeNew:
   "\<lbrakk>g \<oplus> ce \<leadsto> (g2, c);
     g2 \<oplus> te \<leadsto> (g3, t);
     g3 \<oplus> fe \<leadsto> (g4, f);
     s' = meet (stamp g4 t) (stamp g4 f);
-    find_node_and_stamp g4 (ConditionalNode c t f, s') = None;
     n = get_fresh_id g4;
     g' = add_node n (ConditionalNode c t f, s') g4\<rbrakk>
-    \<Longrightarrow> g \<oplus> (ConditionalExpr ce te fe) \<leadsto> (g', n)" |
-
-  UnaryNodeSame:
-  "\<lbrakk>g \<oplus> xe \<leadsto> (g2, x);
-    s' = stamp_unary op (stamp g2 x);
-    find_node_and_stamp g2 (unary_node op x, s') = Some n\<rbrakk>
-    \<Longrightarrow> g \<oplus> (UnaryExpr op xe) \<leadsto> (g2, n)" |
+    \<Longrightarrow> add_expr g (ConditionalExpr ce te fe) (g', n)" |
 
   UnaryNodeNew:
   "\<lbrakk>g \<oplus> xe \<leadsto> (g2, x);
     s' = stamp_unary op (stamp g2 x);
-    find_node_and_stamp g2 (unary_node op x, s') = None;
     n = get_fresh_id g2;
     g' = add_node n (unary_node op x, s') g2\<rbrakk>
-    \<Longrightarrow> g \<oplus> (UnaryExpr op xe) \<leadsto> (g', n)" |
-
-  BinaryNodeSame:
-  "\<lbrakk>g \<oplus> xe \<leadsto> (g2, x);
-    g2 \<oplus> ye \<leadsto> (g3, y);
-    s' = stamp_binary op (stamp g3 x) (stamp g3 y);
-    find_node_and_stamp g3 (bin_node op x y, s') = Some n\<rbrakk>
-    \<Longrightarrow> g \<oplus> (BinaryExpr op xe ye) \<leadsto> (g3, n)" |
+    \<Longrightarrow> add_expr g (UnaryExpr op xe) (g', n)" |
 
   BinaryNodeNew:
   "\<lbrakk>g \<oplus> xe \<leadsto> (g2, x);
     g2 \<oplus> ye \<leadsto> (g3, y);
     s' = stamp_binary op (stamp g3 x) (stamp g3 y);
-    find_node_and_stamp g3 (bin_node op x y, s') = None;
     n = get_fresh_id g3;
     g' = add_node n (bin_node op x y, s') g3\<rbrakk>
-    \<Longrightarrow> g \<oplus> (BinaryExpr op xe ye) \<leadsto> (g', n)" |
+    \<Longrightarrow> add_expr g (BinaryExpr op xe ye) (g', n)" |
 
   AllLeafNodes:
   "\<lbrakk>stamp g n = s;
@@ -413,11 +393,11 @@ inductive
   "\<lbrakk>g \<triangleleft> xe \<leadsto> (g2, x);
     g2 \<triangleleft>\<^sub>L xes \<leadsto> (g3, xs)\<rbrakk>
     \<Longrightarrow> g \<triangleleft>\<^sub>L (xe#xes) \<leadsto> (g3, x#xs)"*)
-
-code_pred (modes: i \<Rightarrow> i \<Rightarrow> o \<Rightarrow> bool as unrepE)
 (*
+code_pred (modes: i \<Rightarrow> i \<Rightarrow> o \<Rightarrow> bool as unrepE)
+
   [show_steps,show_mode_inference,show_intermediate_results] 
-*)  unrep .
+  unrep .
 
 text_raw \<open>\Snip{unrepRules}%
 \begin{center}
@@ -482,5 +462,5 @@ subsection \<open>Maximal Sharing\<close>
 definition maximal_sharing:
   "maximal_sharing g = (\<forall> n\<^sub>1 n\<^sub>2 . n\<^sub>1 \<in> true_ids g \<and> n\<^sub>2 \<in> true_ids g \<longrightarrow> 
       (\<forall> e. (g \<turnstile> n\<^sub>1 \<simeq> e) \<and> (g \<turnstile> n\<^sub>2 \<simeq> e) \<and> (stamp g n\<^sub>1 = stamp g n\<^sub>2) \<longrightarrow> n\<^sub>1 = n\<^sub>2))"
-
+*)
 end
