ROOT
@@ -21,18 +21,18 @@ session Semantics in Semantics = Graph +
   description
     "Semantics of the GraalVM IR"
   options [document = pdf, document_output = "output",
-           show_question_marks = false]
+           show_question_marks = false, quick_and_dirty]
   sessions
     "HOL-Eisbach"
   theories
     IRTreeEval
     IRTreeEvalThms
     TreeToGraph
-    Form
+    (*Form
     IRGraphFrames
     TreeToGraphThms
     IRStepObj
-    IRStepThms
+    IRStepThms*)
   document_files (in "../latex")
     "root.tex"
     "mathpartir.sty"
